VsaIris.lean
@@ -146,6 +146,9 @@ import VsaIris.Vsa.SnpSvf
 import VsaIris.Vsa.SnpSvfConv
 import VsaIris.Vsa.SnpSvfLoop
 import VsaIris.Vsa.SnpSnprintf
+import VsaIris.Vsa.SnpView
+import VsaIris.Vsa.SnpIris
+import VsaIris.Vsa.SnpHoles
 import VsaIris.Interp.IRun
 import VsaIris.Interp.Steps
 import VsaIris.Interp.ITac
